\begin{figure}[ht]
\begin{mathpar}
\inferhref{var}{rule:var}
    {(x : A) \in \Gamma}
    {\typed{\Gamma}{x}{A}}
\and
\inferhref{mor}{rule:mor}
    {f : A \to B \text{ in } \TOT}
    {\typed{\Gamma}{f}{A \to B}}
\and
\inferhref{unit}{rule:unit}{}{\typed{\Gamma}{\unit}{\unitt}}
\\
\inferhref{pair}{rule:pair}
    {\typed{\Gamma}{t}{A} \and \typed{\Gamma}{u}{A}}
    {\typed{\Gamma}{\pair{t}{u}}{A \times B}}
\and
\inferhref{proj1}{rule:proj1}
    {\typed{\Gamma}{t}{A \times B}}
    {\typed{\Gamma}{\projl{t}}{A}}
\and
\inferhref{proj2}{rule:proj2}
    {\typed{\Gamma}{t}{A \times B}}
    {\typed{\Gamma}{\projr{t}}{B}}
\\
\inferhref{abort}{rule:abort}
    {\typed{\Gamma}{t}{\emptyt}}
    {\typed{\Gamma}{\abort{t}}{A}}
\and
\inferhref{inj1}{rule:inj1}
    {\typed{\Gamma}{t}{A}}
    {\typed{\Gamma}{\inl{t}}{A + B}}
\and
\inferhref{inj2}{rule:inj2}
    {\typed{\Gamma}{t}{B}}
    {\typed{\Gamma}{\inr{t}}{A + B}}
\and
\inferhref{case}{rule:case}
    {\typed{\Gamma}{s}{A + B} \and \typed{\Gamma, x : A}{t}{C} \and \typed{\Gamma, y : B}{u}{C}}
    {\typed{\Gamma}{\case{s}{x}{t}{y}{u}}{C}}
\\
\inferhref{lam}{rule:lam}
    {\typed{\Gamma, x : A}{t}{B}}
    {\typed{\Gamma}{\lam{x}{A}{t}}{A \to B}}
\and
\inferhref{app}{rule:app}
    {\typed{\Gamma}{t}{A \to B} \and \typed{\Gamma}{u}{A}}
    {\typed{\Gamma}{\app{t}{u}}{B}}
\\
\inferhref{next}{rule:next}
    {\typed{\Gamma}{t}{A}}
    {\typed{\Gamma}{\nxt{t}}{\Later{A}}}
\and
\inferhref{ap}{rule:ap}
    {\typed{\Gamma}{t}{\Later{(A \to B)}} \and \typed{\Gamma}{u}{\Later{A}}}
    {\typed{\Gamma}{t \ap u}{\Later{B}}}
\and
\inferhref{rec}{rule:rec}
    {\typed{\Gamma, x : \Later{A}}{t}{A}}
    {\typed{\Gamma}{\rec{x}{\Later{A}}{t}}{A}}
\\
\inferhref{true}{rule:true}{}{\typed{\Gamma}{\true}{\Prop}}
\and
\inferhref{false}{rule:false}{}{\typed{\Gamma}{\false}{\Prop}}
\and
\inferhref{eq}{rule:eq}
    {\typed{\Gamma}{t}{A} \and \typed{\Gamma}{u}{A}}
    {\typed{\Gamma}{t =_A u}{\Prop}}
\and
\inferhref{later}{rule:later}
    {\typed{\Gamma}{P}{\Prop}}
    {\typed{\Gamma}{\later{P}}{\Prop}}
\\
\inferhref{conj}{rule:conj}
    {\typed{\Gamma}{P}{\Prop} \and \typed{\Gamma}{Q}{\Prop}}
    {\typed{\Gamma}{P \wedge Q}{\Prop}}
\and
\inferhref{disj}{rule:disj}
    {\typed{\Gamma}{P}{\Prop} \and \typed{\Gamma}{Q}{\Prop}}
    {\typed{\Gamma}{P \vee Q}{\Prop}}
\and
\inferhref{impl}{rule:impl}
    {\typed{\Gamma}{P}{\Prop} \and \typed{\Gamma}{Q}{\Prop}}
    {\typed{\Gamma}{P \impl Q}{\Prop}}
\and
\inferhref{forall}{rule:forall}
    {\typed{\Gamma, x : A}{P}{\Prop}}
    {\typed{\Gamma}{\all{x}{A}{P}}{\Prop}}
\and
\inferhref{exists}{rule:exists}
    {\typed{\Gamma, x : A}{P}{\Prop}}
    {\typed{\Gamma}{\exi{x}{A}{P}}{\Prop}}
\end{mathpar}
\caption{Typing rules for $\lang$}
\label{fig:logic-typing-rules}
\end{figure}

\begin{figure}
\begin{mathpar}
\inferhref{refl}{rule:refl}{}{\entails{\Gamma}{P}{P}}
\and
\inferhref{trans}{rule:trans}
    {\entails{\Gamma}{P}{Q} \and \entails{\Gamma}{Q}{R}}
    {\entails{\Gamma}{P}{R}}
\and
\inferhref{wk}{rule:wk}
    {\entails{\Gamma}{P}{Q}}
    {\entails{\Gamma, x : A}{P}{Q}}
\and
\inferhref{subst}{rule:subst}
    {\entails{\Gamma, x : A}{P}{Q} \and \typed{\Gamma}{t}{A}}
    {\entails{\Gamma}{\subst{P}{x}{t}}{\subst{Q}{x}{t}}}
\\
\inferhref{$\true$-intro}{rule:true-intro}{}{\entails{\Gamma}{P}{\true}}
\and
\inferhref{$\false$-elim}{rule:false-elim}{}{\entails{\Gamma}{\false}{P}}
\and
\inferhref{$\wedge$-intro}{rule:and-intro}
    {\entails{\Gamma}{R}{P} \and \entails{\Gamma}{R}{Q}}
    {\entails{\Gamma}{R}{P \wedge Q}}
\and
\inferhref{$\wedge$-elim-l}{rule:and-elim-l}{}{\entails{\Gamma}{P \wedge Q}{P}}
\and
\inferhref{$\wedge$-elim-r}{rule:and-elim-r}{}{\entails{\Gamma}{P \wedge Q}{Q}}
\\
\inferhref{$\vee$-intro-l}{rule:or-intro-l}{}{\entails{\Gamma}{P}{P \vee Q}}
\and
\inferhref{$\vee$-intro-r}{rule:or-intro-r}{}{\entails{\Gamma}{Q}{P \vee Q}}
\and
\inferhref{$\vee$-elim}{rule:or-elim}
    {\entails{\Gamma}{P}{R} \and \entails{\Gamma}{Q}{R}}
    {\entails{\Gamma}{P \vee Q}{R}}
\and
\inferhref{$\impl$-intro}{rule:impl-intro}
    {\entails{\Gamma}{R \wedge P}{Q}}
    {\entails{\Gamma}{R}{P \impl Q}}
\and
\inferhref{$\impl$-elim}{rule:impl-elim}{}{\entails{\Gamma}{(P \impl Q) \wedge P}{Q}}
\and
\inferhref{$\forall$-intro}{rule:forall-intro}
    {\entails{\Gamma, x : A}{R}{P}}
    {\entails{\Gamma}{R}{\all{x}{A}{P}}}
\and
\inferhref{$\forall$-elim}{rule:forall-elim}
    {\typed{\Gamma}{t}{A}}
    {\entails{\Gamma}{\all{x}{A}{P}}{\subst{P}{x}{t}}}
\and
\inferhref{$\exists$-intro}{rule:exists-intro}
    {\typed{\Gamma}{t}{A}}
    {\entails{\Gamma}{\subst{P}{x}{t}}{\exi{x}{A}{P}}}
\and
\inferhref{$\exists$-elim}{rule:exists-elim}
    {\entails{\Gamma, x : A}{P}{Q}}
    {\entails{\Gamma}{\exi{x}{A}{P}}{Q}}
\and
\inferhref{$\later$-intro}{rule:later-intro2}{}{\entails{\Gamma}{P}{\later{P}}}
\and
\inferhref{$\later$-mono}{rule:later-mono2}
    {\entails{\Gamma}{P}{Q}}
    {\entails{\Gamma}{\later{P}}{\later{Q}}}
\and
\inferhref{$\later$-elim}{rule:later-elim}
    {\valid{}{\later{P}}}
    {\valid{}{P}}
\and
\inferhref{löb}{rule:löb2}
    {\entails{\Gamma}{\later{P}}{P}}
    {\valid{\Gamma}{P}}
\and
\inferhref{$\wedge$-$\later$}{rule:and-later2}{}
    {\entails{\Gamma}{\later{P} \wedge \later{Q}}{\later{(P \wedge Q)}}}
\and
\inferhref{$\later$-$\vee$}{rule:later-or2}{}
    {\entails{\Gamma}{\later{(P \vee Q)}}{\later{P} \vee \later{Q}}}
\and
\inferhref{$\impl$-$\later$}{rule:impl-later2}{}
    {\entails{\Gamma}{\later{P} \impl \later{Q}}{\later{(P \impl Q)}}}
\end{mathpar}
\caption{Structural and logical rules for $\lang$}
\label{fig:structural-logical-rules}
\end{figure}

\begin{figure}
\begin{mathpar}
\inferhref{eq-refl}{rule:eq-refl}
    {\typed{\Gamma}{t}{A}}
    {\equals[A]{\Gamma}{t}{t}}
\and
\inferhref{eq-trans}{rule:eq-trans}
    {\equals[A]{\Gamma}{t}{u} \and \equals[A]{\Gamma}{u}{v}}
    {\equals[A]{\Gamma}{t}{v}}
\and
\inferhref{eq-sym}{rule:eq-sym}
    {\equals[A]{\Gamma}{t}{u}}
    {\equals[A]{\Gamma}{u}{t}}
\\
\inferhref{eq-prop}{rule:eq-prop}
    {}
    {\entails{\Gamma}{P =_{\Prop} Q \wedge P}{Q}}
\and
\inferhref{propext}{rule:propext}
    {}
    {\entails{\Gamma}{(P \impl Q) \wedge (Q \impl P)}{P =_{\Prop} Q}}
\and
\inferhref{$\unitt$-$\eta$}{rule:top-eta}
    {\typed{\Gamma}{t}{\unitt}}
    {\equals[\unitt]{\Gamma}{t}{\unit}}
\\
\inferhref{$\times$-$\beta$-1}{rule:prod-beta-1}
    {\typed{\Gamma}{t}{A} \and \typed{\Gamma}{u}{B}}
    {\equals[A]{\Gamma}{\projl{\pair{t}{u}}}{t}}
\and
\inferhref{$\times$-$\beta$-2}{rule:prod-beta-2}
    {\typed{\Gamma}{t}{A} \and \typed{\Gamma}{u}{B}}
    {\equals[B]{\Gamma}{\projr{\pair{t}{u}}}{u}}
\and
\inferhref{$\times$-$\eta$}{rule:prod-eta}
    {\typed{\Gamma}{t}{A \times B}}
    {\equals[A \times B]{\Gamma}{\pair{\projl{t}}{\projr{t}}}{t}}
\\
\inferhref{$+$-$\beta$-1}{rule:sum-beta-1}
    {\typed{\Gamma}{t}{A} \and \typed{\Gamma, x : A}{u}{C}
        \and \typed{\Gamma, y : B}{v}{C}}
    {\equals[C]{\Gamma}{\case{\inl{t}}{x}{u}{y}{v}}{\subst{u}{x}{t}}}
\and
\inferhref{$+$-$\beta$-2}{rule:sum-beta-2}
    {\typed{\Gamma}{t}{B} \and \typed{\Gamma, x : A}{u}{C}
        \and \typed{\Gamma, y : B}{v}{C}}
    {\equals[C]{\Gamma}{\case{\inr{t}}{x}{u}{y}{v}}{\subst{v}{y}{t}}}
\\
\inferhref{$\to$-$\beta$}{rule:fun-beta}
    {\typed{\Gamma, x : A}{t}{B} \and \typed{\Gamma}{u}{A}}
    {\equals[B]{\Gamma}{\app{(\lam{x}{A}{t})}{u}}{\subst{t}{x}{u}}}
\and
\inferhref{$\to$-$\eta$}{rule:fun-eta}
    {\typed{\Gamma}{t}{A \to B} \and (x : A) \notin \Gamma}
    {\equals[A \to B]{\Gamma}{\lam{x}{A}{\app{t}{x}}}{t}}
\and
\inferhref{$\ap$-next}{rule:ap-next2}
    {\typed{\Gamma}{t}{A \to B} \and \typed{\Gamma}{u}{A}}
    {\equals[\Later{B}]{\Gamma}{\nxt{t} \ap \nxt{u}}{\nxt{(\app{t}{u})}}}
\and
\inferhref{$\ap$-comp}{rule:ap-comp2}
    {\typed{\Gamma}{f}{\Later{(B \to C)}} \and \typed{\Gamma}{g}{\Later{(A \to B)}} 
        \and \typed{\Gamma}{t}{\Later{A}}}
    {\equals[\Later{C}]{\Gamma}{f \ap (g \ap t)}{\nxt{\name{comp}} \ap f \ap g \ap t}}
\and
\inferhref{fix-$\beta$}{rule:fix-beta2}
    {\typed{\Gamma, x : \Later{A}}{t}{A}}
    {\equals[A]{\Gamma}{\rec{x}{\Later{A}}{t}}
        {\subst{t}{x}{\nxt{(\rec{x}{\Later{A}}{t})}}}}
\and
\inferhref{fix-$\eta$}{rule:fix-eta}
    {\typed{\Gamma, x : \Later{A}}{t}{A} \and \typed{\Gamma}{z}{A} \and
        \equals{\Gamma}{z}{\subst{t}{x}{\nxt{z}}}}
    {\equals[A]{\Gamma}{z}{\rec{x}{\Later{A}}{t}}}
\\
\inferhref{$\later$-eq}{rule:later-eq2}{}
    {\equiv{\Gamma}{\later{(t =_A u)}}{\nxt{t} =_{\Later{A}} \nxt{u}}}
\end{mathpar}
\caption{Equality rules in $\lang$. $\name{comp} : (B \to C) \to (A \to B) \to A \to C$ is function composition. Congruence cases are omitted.}
\label{fig:logic-equalities}
\end{figure}
